internal/examples/semantics/strings.go
@@ -1,0 +1,33 @@
+package semantics
+
+import "github.com/tchajed/goose/machine"
+
+func stringAppend(s string, x uint64) string {
+	return s + machine.UInt64ToString(x)
+}
+
+func stringLength(s string) uint64 {
+	return uint64(len(s))
+}
+
+func testStringAppend() bool {
+	var ok = true
+	var s = "123"
+
+	var y = stringAppend(s, 45)
+	return ok && (y == "12345")
+}
+
+func testStringLength() bool {
+	var ok = true
+	var s = ""
+
+	ok = ok && (uint64(len(s)) == 0)
+
+	s = stringAppend(s, 1)
+	ok = ok && (uint64(len(s)) == 1)
+
+	s = stringAppend(s, 23)
+
+	return ok && (uint64(len(s)) == 3)
+}
